PAC: more function and switch to multisets for address

PAC_Checker2/EPAC_Perfectly_Shared_Vars.thy
@@ -5,13 +5,17 @@ begin
 
 text \<open>We now introduce sharing of variables to make a more efficient representation possible.\<close>
 
-section \<open>Definition\<close>
+section \<open>Perfectly sharing of elements\<close>
+
+subsection \<open>Definition\<close>
+  
+type_synonym ('nat, 'string) shared_vars = \<open>'string multiset \<times> ('nat, 'string) fmap \<times> ('string, 'nat) fmap\<close>
 
 definition perfectly_shared_vars
-  :: \<open>'nat set \<Rightarrow> 'string set \<Rightarrow> ('nat, 'string) fmap \<times> ('string, 'nat) fmap  \<Rightarrow> bool\<close>
+  :: \<open>'string multiset \<Rightarrow>  ('nat, 'string) shared_vars \<Rightarrow> bool\<close>
 where
-  \<open>perfectly_shared_vars D \<V> = (\<lambda>(V, V').
-  D \<subseteq> set_mset (dom_m V) \<and> set_mset (dom_m V') = \<V> \<and>
+  \<open>perfectly_shared_vars \<V> = (\<lambda>(\<D>, V, V').
+  set_mset (dom_m V') = set_mset \<V> \<and> \<D> = \<V> \<and> 
   (\<forall>i \<in>#dom_m V. fmlookup V' (the (fmlookup V i)) = Some i) \<and>
   (\<forall>str \<in>#dom_m V'. fmlookup V (the (fmlookup V' str)) = Some str) \<and>
   (\<forall>i j. i\<in>#dom_m V \<longrightarrow> j\<in>#dom_m V \<longrightarrow> (fmlookup V i = fmlookup V j \<longleftrightarrow> i = j)))\<close>
@@ -20,9 +24,8 @@ abbreviation fmlookup_direct :: \<open>('a, 'b) fmap \<Rightarrow> 'a \<Rightarr
   \<open>fmlookup_direct A b \<equiv> the (fmlookup A b)\<close>
 
 lemma perfectly_shared_vars_simps:
-  assumes \<open>perfectly_shared_vars D \<V> (VV')\<close>
-  shows \<open>str \<in> \<V> \<longleftrightarrow> str \<in># dom_m (snd VV')\<close> and
-    \<open>i \<in> D \<Longrightarrow> i \<in># dom_m (fst VV')\<close>
+  assumes \<open>perfectly_shared_vars \<V> (VV')\<close>
+  shows \<open>str \<in># \<V> \<longleftrightarrow> str \<in># dom_m (snd (snd VV'))\<close>
   using assms
   unfolding perfectly_shared_vars_def
   apply auto
@@ -31,14 +34,14 @@ lemma perfectly_shared_vars_simps:
 lemma perfectly_shared_add_new_var:
   fixes V :: \<open>('nat, 'string) fmap\<close> and
     v :: \<open>'string\<close>
-  assumes \<open>perfectly_shared_vars D \<V> (V, V')\<close> and
-    \<open>v \<notin> \<V>\<close> and
+  assumes \<open>perfectly_shared_vars \<V> (D, V, V')\<close> and
+    \<open>v \<notin># \<V>\<close> and
     k_notin[simp]: \<open>k \<notin># dom_m V\<close>
-  shows \<open>perfectly_shared_vars D (insert v \<V>) (fmupd k v V, fmupd v k V')\<close>
+  shows \<open>perfectly_shared_vars (add_mset v \<V>) (add_mset v D, fmupd k v V, fmupd v k V')\<close>
 proof -
   have
-    DV: \<open>D \<subseteq> set_mset (dom_m V)\<close> and
-    V'\<V>: \<open>set_mset (dom_m V') = \<V>\<close> and
+    DV[simp]: \<open>D = \<V>\<close> and
+    V'\<V>: \<open>set_mset (dom_m V') = set_mset \<V>\<close> and
     map: \<open>\<And>i. i \<in>#dom_m V \<Longrightarrow> fmlookup V' (the (fmlookup V i)) = Some i\<close> and
     map_str: \<open>\<And>str. str \<in>#dom_m V' \<Longrightarrow> fmlookup V (the (fmlookup V' str)) = Some str\<close> and
     perfect: \<open>\<And>i j. i\<in>#dom_m V \<Longrightarrow> j\<in>#dom_m V \<Longrightarrow> fmlookup V i = fmlookup V j \<longleftrightarrow> i = j\<close>
@@ -49,9 +52,9 @@ proof -
   show ?thesis
     unfolding perfectly_shared_vars_def prod.simps
   proof (intro conjI allI ballI impI)
-    show \<open>D \<subseteq> set_mset (dom_m (fmupd k v V))\<close>
+    show \<open>add_mset v D = add_mset v \<V>\<close>
       using DV by auto
-    show \<open>set_mset (dom_m (fmupd v k V')) = insert v \<V>\<close>
+    show \<open>set_mset (dom_m (fmupd v k V')) = set_mset (add_mset v \<V>)\<close>
       using V'\<V> in_remove1_mset_neq by fastforce
  
     show \<open>fmlookup (fmupd v k V') (fmupd k v V \<propto> i) = Some i\<close>
@@ -77,15 +80,13 @@ proof -
   qed
 qed
 
-lemma perfectly_shared_add_del_vars:
-  fixes V :: \<open>('nat, 'string) fmap\<close> and
-    v :: \<open>'string\<close>
-  assumes \<open>perfectly_shared_vars D \<V> (V, V')\<close> and
-    \<open>D' \<subseteq> D\<close>
-  shows \<open>perfectly_shared_vars D' (\<V>) (V, V')\<close>
+lemma perfectly_shared_vars_remove_update:
+  assumes \<open>perfectly_shared_vars (add_mset v \<V>) (D, V, V')\<close> and
+    \<open>v \<notin># \<V>\<close>
+  shows \<open>perfectly_shared_vars  \<V> (remove1_mset v D, fmdrop (V' \<propto> v) V, fmdrop v V')\<close>
   using assms
   unfolding perfectly_shared_vars_def
-  by blast
+  by (fastforce simp: distinct_mset_dom distinct_mset_remove1_All)
 
 
 section \<open>Refinement\<close>
@@ -93,35 +94,55 @@ section \<open>Refinement\<close>
 datatype memory_allocation =
   Allocated | alloc_failed: Mem_Out
 
-type_synonym ('nat, 'string) shared_vars = \<open>('nat, 'string) fmap \<times> ('string, 'nat) fmap\<close>
-type_synonym ('nat, 'string) vars = \<open>'nat set \<times> 'string set\<close>
+type_synonym ('nat, 'string) vars = \<open>'string multiset\<close>
 
 definition perfectly_shared_var_rel :: \<open>('nat,'string) shared_vars \<Rightarrow> ('nat \<times> 'string) set\<close> where
-  \<open>perfectly_shared_var_rel = (\<lambda>(\<V>, \<V>'). br (\<lambda>i. \<V> \<propto> i) (\<lambda>i. i \<in># dom_m \<V>))\<close>
+  \<open>perfectly_shared_var_rel = (\<lambda>(\<D>, \<V>, \<V>'). br (\<lambda>i. \<V> \<propto> i) (\<lambda>i. i \<in># dom_m \<V>))\<close>
 
 definition perfectly_shared_vars_rel :: \<open>(('nat,'string) shared_vars \<times> ('nat, 'string) vars) set\<close>
 where
-  \<open>perfectly_shared_vars_rel = {(\<A>, (\<D>, \<V>)). perfectly_shared_vars \<D> \<V> \<A>}\<close>
+  \<open>perfectly_shared_vars_rel = {(\<A>, \<V>). perfectly_shared_vars \<V> \<A>}\<close>
+
+definition import_variableS
+  :: \<open>'string \<Rightarrow> ('nat, 'string) shared_vars \<Rightarrow>
+  (memory_allocation \<times> ('nat, 'string) shared_vars \<times> 'nat) nres\<close>
+where
+  \<open>import_variableS v = (\<lambda>(\<D>, \<V>, \<V>'). do {
+    (mem, k) \<leftarrow> SPEC(\<lambda>(mem, k::'nat). \<not>alloc_failed mem \<longrightarrow> k \<notin># dom_m \<V>);
+    if alloc_failed mem then do {k \<leftarrow> RES (UNIV :: 'nat set); RETURN (mem, (\<D>, \<V>, \<V>'), k)}
+    else RETURN (Allocated, (add_mset v \<D>, fmupd k v \<V>, fmupd v k \<V>'), k)
+  })\<close>
 
 definition import_variable
-  :: \<open>'string \<Rightarrow> ('nat, 'string) fmap \<times> ('string, 'nat) fmap \<Rightarrow>
-  (memory_allocation \<times> ('nat, 'string) fmap \<times> ('string, 'nat) fmap) nres\<close>
-where
-  \<open>import_variable v = (\<lambda>(\<V>, \<V>'). do {
-    (mem, k) \<leftarrow> SPEC(\<lambda>(mem, k::'nat). \<not>alloc_failed mem \<longrightarrow> k \<notin># dom_m \<V>);
-    if alloc_failed mem then RETURN (mem, (\<V>, \<V>'))
-    else RETURN (Allocated, (fmupd k v \<V>, fmupd v k \<V>'))
+  :: \<open>'string \<Rightarrow> ('nat, 'string) vars \<Rightarrow> (memory_allocation \<times> ('nat, 'string) vars \<times> 'string) nres\<close>
+  where
+  \<open>import_variable v = (\<lambda>\<V>. do {
+     ASSERT(v \<notin># \<V>);
+     SPEC(\<lambda>(mem, \<V>', k::'string). \<not>alloc_failed mem \<longrightarrow> \<V>' = add_mset k \<V> \<and> k = v)
   })\<close>
 
 definition is_new_variableS :: \<open>'string \<Rightarrow> ('nat, 'string) shared_vars \<Rightarrow> bool nres\<close> where
-  \<open>is_new_variableS v = (\<lambda>(\<V>, \<V>').
+  \<open>is_new_variableS v = (\<lambda>(\<D>, \<V>, \<V>').
   RETURN (v \<notin># dom_m \<V>')
   )\<close>
 
 definition is_new_variable :: \<open>'string \<Rightarrow> ('nat, 'string) vars \<Rightarrow> bool nres\<close> where
-  \<open>is_new_variable v = (\<lambda>(\<V>, \<V>').
-    RETURN (v \<notin> \<V>')
+  \<open>is_new_variable v = (\<lambda>\<V>'.
+    RETURN (v \<notin># \<V>')
   )\<close>
+
+
+lemma import_variableS_import_variable:
+  fixes \<V> :: \<open>('nat, 'string) vars\<close>
+  assumes \<open>(\<A>, \<V>) \<in> perfectly_shared_vars_rel\<close> and \<open>(v, v') \<in> Id\<close>
+  shows \<open>import_variableS v \<A> \<le> \<Down>({((mem, \<A>', i), (mem', \<V>', j)). mem = mem' \<and>
+    (\<A>', \<V>') \<in> perfectly_shared_vars_rel \<and> (\<not>alloc_failed mem' \<longrightarrow> (i, j) \<in> perfectly_shared_var_rel \<A>') \<and>
+    (\<forall>xs. xs \<in> perfectly_shared_var_rel \<A> \<longrightarrow> xs \<in> perfectly_shared_var_rel \<A>')}) (import_variable v' \<V>)\<close>
+  using assms
+  unfolding import_variableS_def import_variable_def
+  by (refine_vcg lhs_step_If)
+   (auto intro!: RETURN_RES_refine simp:  perfectly_shared_add_new_var perfectly_shared_vars_rel_def
+    perfectly_shared_var_rel_def br_def)
 
 lemma is_new_variable_spec:
   assumes \<open>(\<A>, \<D>\<V>) \<in> perfectly_shared_vars_rel\<close> \<open>(v,v') \<in> Id\<close>
@@ -134,13 +155,13 @@ lemma is_new_variable_spec:
 
 definition get_var_name :: \<open>('nat, 'string) vars \<Rightarrow> 'string \<Rightarrow>  'string nres\<close> where
   \<open>get_var_name \<V> x = do {
-    ASSERT(x \<in> snd \<V>);
+    ASSERT(x \<in># \<V>);
     RETURN x
   }\<close>
 definition get_var_nameS :: \<open>('nat, 'string) shared_vars \<Rightarrow> 'string \<Rightarrow> 'nat nres\<close> where
   \<open>get_var_nameS \<V> x = do {
-    ASSERT(x \<in># dom_m (snd \<V>));
-    RETURN (snd \<V> \<propto> x)
+    ASSERT(x \<in># dom_m (snd (snd \<V>)));
+    RETURN (snd (snd \<V>) \<propto> x)
   }\<close>
 
 lemma get_var_nameS_spec:
@@ -156,18 +177,17 @@ lemma get_var_nameS_spec:
     perfectly_shared_vars_rel_def perfectly_shared_vars_simps br_def
     intro!: ASSERT_leI)
   apply (simp_all add: perfectly_shared_vars_def in_dom_m_lookup_iff)
-  using indom_mI apply force
-  by (meson indom_mI)
+  done
 
 abbreviation perfectly_shared_monom
   :: \<open>('nat,'string) shared_vars \<Rightarrow> ('nat list \<times> 'string list) set\<close>
 where
   \<open>perfectly_shared_monom \<V> \<equiv> \<langle>perfectly_shared_var_rel \<V>\<rangle>list_rel \<close>
 
-definition import_monomS
+definition import_monom_no_newS
   :: \<open>('nat, 'string) shared_vars \<Rightarrow> 'string list \<Rightarrow> (bool \<times> 'nat list) nres\<close>
 where
-  \<open>import_monomS \<A> xs = do {
+  \<open>import_monom_no_newS \<A> xs = do {
   (new, _, xs) \<leftarrow> WHILE\<^sub>T (\<lambda>(new, xs, _). \<not>new \<and> xs \<noteq> [])
     (\<lambda>(_, xs, ys). do {
       ASSERT(xs \<noteq> []);
@@ -184,10 +204,10 @@ where
   RETURN (new, xs)
  }\<close>
 
-definition import_monom
+definition import_monom_no_new
   :: \<open>('nat, 'string) vars \<Rightarrow> 'string list \<Rightarrow> (bool \<times> 'string list) nres\<close>
 where
-  \<open>import_monom \<A> xs = do {
+  \<open>import_monom_no_new \<A> xs = do {
   (new, _, xs) \<leftarrow> WHILE\<^sub>T (\<lambda>(new, xs, _). \<not>new \<and> xs \<noteq> [])
   (\<lambda>(_, xs, ys). do {
     ASSERT(xs \<noteq> []);
@@ -204,14 +224,14 @@ where
   RETURN (new, xs)
 }\<close>
 
-lemma import_monom_spec:
-  shows \<open>import_monom \<A> xs \<le> \<Down> Id
-    (SPEC(\<lambda>(new, ys). (new \<longrightarrow> \<not>set xs \<subseteq> snd \<A>) \<and>
+lemma import_monom_no_new_spec:
+  shows \<open>import_monom_no_new \<A> xs \<le> \<Down> Id
+    (SPEC(\<lambda>(new, ys). (new \<longrightarrow> \<not>set xs \<subseteq> set_mset \<A>) \<and>
       \<not>new \<longrightarrow> ys = xs))\<close>
-  unfolding import_monom_def is_new_variable_def get_var_name_def
+  unfolding import_monom_no_new_def is_new_variable_def get_var_name_def
   apply (refine_vcg
-    WHILET_rule[where I = \<open>(\<lambda>(new, ys, zs). (\<not>new \<longrightarrow> xs = zs @ ys) \<and> (\<not>new \<longrightarrow> set zs \<subseteq> snd \<A>) \<and>
-     (new \<longrightarrow> \<not>set xs \<subseteq> snd \<A>))\<close> and
+    WHILET_rule[where I = \<open>(\<lambda>(new, ys, zs). (\<not>new \<longrightarrow> xs = zs @ ys) \<and> (\<not>new \<longrightarrow> set zs \<subseteq> set_mset \<A>) \<and>
+     (new \<longrightarrow> \<not>set xs \<subseteq> set_mset \<A>))\<close> and
     R = \<open>measure (\<lambda>(_, ys, _). length ys)\<close>])
   subgoal by auto
   subgoal by auto
@@ -230,12 +250,12 @@ lemma import_monom_spec:
   subgoal by auto
   done
 
-lemma import_monomS_import_monom:
+lemma import_monom_no_newS_import_monom_no_new:
   assumes \<open>(\<A>, \<V>\<D>) \<in> perfectly_shared_vars_rel\<close> \<open>(xs, xs') \<in> Id\<close>
-  shows \<open>import_monomS \<A> xs \<le> \<Down>(bool_rel \<times>\<^sub>r perfectly_shared_monom \<A>)
-    (import_monom \<V>\<D> xs')\<close>
+  shows \<open>import_monom_no_newS \<A> xs \<le> \<Down>(bool_rel \<times>\<^sub>r perfectly_shared_monom \<A>)
+    (import_monom_no_new \<V>\<D> xs')\<close>
   using assms
-  unfolding import_monom_def import_monomS_def
+  unfolding import_monom_no_new_def import_monom_no_newS_def
   apply (refine_rcg WHILET_refine[where R = \<open>bool_rel \<times>\<^sub>r \<langle>Id\<rangle>list_rel \<times>\<^sub>r perfectly_shared_monom \<A>\<close>]
     is_new_variable_spec get_var_nameS_spec)
   subgoal by auto
@@ -251,15 +271,15 @@ lemma import_monomS_import_monom:
   subgoal by auto
   done
 
- definition import_polyS
+ definition import_poly_no_newS
   :: \<open>('nat, 'string) shared_vars \<Rightarrow> ('string list \<times> 'a) list \<Rightarrow> (bool \<times> ('nat list \<times> 'a)list) nres\<close>
 where
-  \<open>import_polyS \<A> xs = do {
+  \<open>import_poly_no_newS \<A> xs = do {
   (new, _, xs) \<leftarrow> WHILE\<^sub>T (\<lambda>(new, xs, _). \<not>new \<and> xs \<noteq> [])
     (\<lambda>(_, xs, ys). do {
       ASSERT(xs \<noteq> []);
       let (x, n) = hd xs;
-      (b, x) \<leftarrow> import_monomS \<A> x;
+      (b, x) \<leftarrow> import_monom_no_newS \<A> x;
       if b
       then RETURN (True, tl xs, ys)
       else do {
@@ -270,15 +290,15 @@ where
   RETURN (new, xs)
  }\<close>
 
-definition import_poly
+definition import_poly_no_new
   :: \<open>('nat, 'string) vars \<Rightarrow> ('string list \<times> 'a) list \<Rightarrow> (bool \<times> ('string list \<times> 'a) list) nres\<close>
 where
-  \<open>import_poly \<A> xs = do {
+  \<open>import_poly_no_new \<A> xs = do {
   (new, _, xs) \<leftarrow> WHILE\<^sub>T (\<lambda>(new, xs, _). \<not>new \<and> xs \<noteq> [])
   (\<lambda>(_, xs, ys). do {
     ASSERT(xs \<noteq> []);
     let (x, n) = hd xs;
-    (b, x) \<leftarrow> import_monom \<A> x;
+    (b, x) \<leftarrow> import_monom_no_new \<A> x;
     if b
     then RETURN (True, tl xs, ys)
       else do {
@@ -290,15 +310,15 @@ where
 }\<close>
 
 
-lemma import_polyS_import_poly:
+lemma import_poly_no_newS_import_poly_no_new:
   assumes \<open>(\<A>, \<V>\<D>) \<in> perfectly_shared_vars_rel\<close> \<open>(xs, xs') \<in> Id\<close>
-  shows \<open>import_polyS \<A> xs \<le> \<Down>(bool_rel \<times>\<^sub>r \<langle>perfectly_shared_monom \<A> \<times>\<^sub>r Id\<rangle>list_rel)
-    (import_poly \<V>\<D> xs')\<close>
+  shows \<open>import_poly_no_newS \<A> xs \<le> \<Down>(bool_rel \<times>\<^sub>r \<langle>perfectly_shared_monom \<A> \<times>\<^sub>r Id\<rangle>list_rel)
+    (import_poly_no_new \<V>\<D> xs')\<close>
   using assms
-  unfolding import_poly_def import_polyS_def
+  unfolding import_poly_no_new_def import_poly_no_newS_def
   apply (refine_rcg WHILET_refine[where
     R = \<open>bool_rel \<times>\<^sub>r \<langle>Id\<rangle>list_rel \<times>\<^sub>r \<langle>perfectly_shared_monom \<A> \<times>\<^sub>r Id\<rangle>list_rel\<close>]
-    import_monomS_import_monom)
+    import_monom_no_newS_import_monom_no_new)
   subgoal by auto
   subgoal by auto
   subgoal by auto
@@ -309,4 +329,252 @@ lemma import_polyS_import_poly:
   subgoal by auto
   done
 
+definition import_monomS
+  :: \<open>('nat, 'string) shared_vars \<Rightarrow> 'string list \<Rightarrow> (_ \<times> 'nat list \<times> ('nat, 'string) shared_vars) nres\<close>
+where
+  \<open>import_monomS \<A> xs = do {
+  (new, _, xs, \<A>) \<leftarrow> WHILE\<^sub>T (\<lambda>(mem, xs, _, _). \<not>alloc_failed mem \<and> xs \<noteq> [])
+    (\<lambda>(_, xs, ys, \<A>). do {
+      ASSERT(xs \<noteq> []);
+      let x = hd xs;
+      b \<leftarrow> is_new_variableS x \<A>;
+      if b
+      then do {
+        (mem, \<A>, x) \<leftarrow> import_variableS x \<A>;
+        if alloc_failed mem
+        then RETURN (mem, xs, ys, \<A>)
+        else RETURN (mem, tl xs, ys @ [x], \<A>)
+      }
+      else do {
+        x \<leftarrow> get_var_nameS \<A> x;
+        RETURN (Allocated, tl xs, ys @ [x], \<A>)
+       }
+    })
+    (Allocated, xs, [], \<A>);
+  RETURN (new, xs, \<A>)
+ }\<close>
+
+definition import_monom
+  :: \<open>('nat, 'string) vars \<Rightarrow> 'string list \<Rightarrow> (memory_allocation \<times> 'string list \<times> ('nat, 'string) vars) nres\<close>
+where
+  \<open>import_monom \<A> xs = do {
+  (new, _, xs, \<A>) \<leftarrow> WHILE\<^sub>T (\<lambda>(new, xs, _, _). \<not>alloc_failed new \<and> xs \<noteq> [])
+  (\<lambda>(mem, xs, ys, \<A>). do {
+  ASSERT(xs \<noteq> []);
+  let x = hd xs;
+    b \<leftarrow> is_new_variable x \<A>;
+    if b
+  then do {
+    (mem, \<A>, x) \<leftarrow> import_variable x \<A>;
+    if alloc_failed mem
+    then RETURN (mem, xs, ys, \<A>)
+    else RETURN (mem, tl xs, ys @ [x], \<A>)
+    }
+    else do {
+    x \<leftarrow> get_var_name \<A> x;
+    RETURN (mem, tl xs, ys @ [x], \<A>)
+    }
+    })
+    (Allocated, xs, [], \<A>);
+    RETURN (new, xs, \<A>)
+    }\<close>
+
+lemma import_monom_spec:
+  shows \<open>import_monom \<A> xs \<le> \<Down> Id
+    (SPEC(\<lambda>(new, ys, \<A>'). \<not>alloc_failed new \<longrightarrow> ys = xs \<and> set_mset \<A>' = set_mset \<A> \<union> set xs))\<close>
+proof -
+  define I where
+    [simp]: \<open>I = (\<lambda>(new, ys, zs, \<A>'). \<not>alloc_failed new \<longrightarrow> (xs = zs @ ys \<and> set_mset \<A>' = set_mset \<A> \<union> set zs))\<close>
+  show ?thesis
+  unfolding import_monom_def is_new_variable_def get_var_name_def import_variable_def
+  apply (refine_vcg
+    WHILET_rule[where I = \<open>I\<close> and
+    R = \<open>measure (\<lambda>(mem, ys, _). (if alloc_failed mem then 0 else 1) + length ys)\<close>])
+  subgoal by auto
+  subgoal by auto
+  subgoal by auto
+  subgoal by (auto simp: neq_Nil_conv)
+  subgoal by auto
+  subgoal by auto
+  subgoal by auto
+  subgoal by auto
+  subgoal by auto
+  subgoal by auto
+  subgoal by auto
+  subgoal by auto
+  done
+qed
+
+definition import_polyS
+  :: \<open>('nat, 'string) shared_vars \<Rightarrow> ('string list \<times> 'a) list \<Rightarrow> 
+    (memory_allocation \<times> ('nat list \<times> 'a)list \<times> ('nat, 'string) shared_vars) nres\<close>
+  where
+  \<open>import_polyS \<A> xs = do {
+  (mem,_, xs, \<A>) \<leftarrow> WHILE\<^sub>T (\<lambda>(mem, xs, _, _). \<not>alloc_failed mem \<and> xs \<noteq> [])
+    (\<lambda>(mem, xs, ys, \<A>). do {
+      ASSERT(xs \<noteq> []);
+      let (x, n) = hd xs;
+      (mem, x, \<A>) \<leftarrow> import_monomS \<A> x;
+      if alloc_failed mem
+      then RETURN (mem, xs, ys, \<A>)
+      else do {
+       RETURN (mem, tl xs, ys @ [(x, n)], \<A>)
+      }
+    }) 
+    (Allocated, xs, [], \<A>);
+   RETURN (mem, xs, \<A>)
+ }\<close>
+
+definition import_poly
+  :: \<open>('nat, 'string) vars \<Rightarrow> ('string list \<times> 'a) list \<Rightarrow>
+        (memory_allocation \<times> ('string list \<times> 'a) list \<times> ('nat, 'string)vars) nres\<close>
+  where
+  \<open>import_poly \<A> xs = do {
+  (new, _, xs, \<A>) \<leftarrow> WHILE\<^sub>T (\<lambda>(new, xs, _). \<not>alloc_failed new \<and> xs \<noteq> [])
+  (\<lambda>(_, xs, ys, \<A>). do {
+    ASSERT(xs \<noteq> []);
+    let (x, n) = hd xs;
+    (b, x, \<A>) \<leftarrow> import_monom \<A> x;
+    if alloc_failed b
+    then RETURN (b, xs, ys, \<A>)
+    else do {
+      RETURN (Allocated, tl xs, ys @ [(x, n)], \<A>)
+    }
+  })
+  (Allocated, xs, [], \<A>);
+  RETURN (new, xs, \<A>)
+}\<close>
+
+lemma import_poly_spec:
+  fixes \<A> :: \<open>('nat, 'string) vars\<close>
+  shows \<open>import_poly \<A> xs \<le> \<Down> Id
+    (SPEC(\<lambda>(new, ys, \<A>'). \<not>alloc_failed new \<longrightarrow> ys = xs \<and> set_mset \<A>' = set_mset \<A> \<union> \<Union>(set `fst ` set xs)))\<close>
+proof -
+  define I where
+    [simp]: \<open>I = (\<lambda>(new, ys, zs, \<A>'). \<not>alloc_failed new \<longrightarrow> (xs = zs @ ys \<and>
+       set_mset \<A>' = set_mset \<A> \<union> \<Union>(set ` fst ` set zs)))\<close>
+  show ?thesis
+    unfolding import_poly_def is_new_variable_def get_var_name_def import_variable_def
+    apply (refine_vcg import_monom_spec[THEN order_trans]
+      WHILET_rule[where I = \<open>I\<close> and
+      R = \<open>measure (\<lambda>(mem, ys, _). (if alloc_failed mem then 0 else 1) + length ys)\<close>])
+    subgoal by auto
+    subgoal by auto
+    subgoal by auto
+    subgoal by (auto simp: neq_Nil_conv)
+    subgoal by auto
+    subgoal by auto
+    done
+qed
+
+lemma list_rel_append_single: \<open>(xs, ys) \<in> \<langle>R\<rangle>list_rel \<Longrightarrow> (x, y) \<in> R \<Longrightarrow> (xs @ [x], ys @ [y]) \<in> \<langle>R\<rangle>list_rel\<close>
+  by (meson list_rel_append1 list_rel_simp(4) refine_list(1))
+
+lemma list_rel_mono: \<open>A \<in> \<langle>R\<rangle>list_rel \<Longrightarrow> (\<And>xs. xs \<in> R \<Longrightarrow> xs \<in> R') \<Longrightarrow> A \<in> \<langle>R'\<rangle>list_rel\<close>
+  unfolding list_rel_def
+  apply (cases A)
+  by (simp add: list_all2_mono)
+
+lemma import_monomS_import_monom:
+  fixes \<V>\<D> :: \<open>('nat, 'string) vars\<close> and \<A>\<^sub>0 :: \<open>('nat, 'string)shared_vars\<close> and xs xs' :: \<open>'string list\<close>
+  assumes \<open>(\<A>\<^sub>0, \<V>\<D>) \<in> perfectly_shared_vars_rel\<close> \<open>(xs, xs') \<in> \<langle>Id\<rangle>list_rel\<close>
+  shows \<open>import_monomS \<A>\<^sub>0 xs \<le> \<Down> {((mem, xs\<^sub>0, \<A>), (mem', ys\<^sub>0, \<A>')). mem = mem' \<and> 
+    (\<A>, \<A>') \<in> perfectly_shared_vars_rel \<and>  (\<not>alloc_failed mem \<longrightarrow> (xs\<^sub>0, ys\<^sub>0) \<in> perfectly_shared_monom \<A>)\<and>
+    (\<not>alloc_failed mem \<longrightarrow> (\<forall>xs. xs \<in> perfectly_shared_monom \<A>\<^sub>0 \<longrightarrow> xs \<in> perfectly_shared_monom \<A>))}
+    (import_monom \<V>\<D> xs')\<close>
+  using assms
+  unfolding import_monom_def import_monomS_def
+  apply (refine_rcg WHILET_refine[where
+    R = \<open>{((mem::memory_allocation, xs\<^sub>0::'string list, zs\<^sub>0::'nat list,  \<A> :: ('nat, 'string)shared_vars),
+    (mem', ys\<^sub>0::'string list, zs\<^sub>0'::'string list, \<A>' :: ('nat, 'string)vars)). mem = mem' \<and>
+    (\<A>, \<A>') \<in> perfectly_shared_vars_rel \<and> (\<not>alloc_failed mem \<longrightarrow> (zs\<^sub>0, zs\<^sub>0') \<in> perfectly_shared_monom \<A>) \<and>
+    (xs\<^sub>0, ys\<^sub>0) \<in> \<langle>Id\<rangle>list_rel \<and>
+    (\<not>alloc_failed mem \<longrightarrow> (\<forall>xs. xs \<in> perfectly_shared_monom \<A>\<^sub>0 \<longrightarrow> xs \<in> perfectly_shared_monom \<A>))}\<close>]
+    import_variableS_import_variable
+    is_new_variable_spec get_var_nameS_spec)
+  subgoal by auto
+  subgoal
+    by auto
+  subgoal
+    by auto 
+  subgoal by auto
+  subgoal by auto
+  subgoal by auto
+  subgoal by auto
+  subgoal by auto
+  subgoal by auto
+  subgoal by auto
+  subgoal apply (auto intro!: list_rel_append_single intro: list_rel_mono)
+    by (metis (full_types) EPAC_Perfectly_Shared_Vars.list_rel_mono surj_pair)
+  subgoal by auto
+  subgoal by auto
+  subgoal using memory_allocation.exhaust_disc  by (auto intro!: list_rel_append_single intro: list_rel_mono)
+  subgoal by auto
+  done
+
+lemma import_polyS_import_poly:
+  assumes \<open>(\<A>, \<V>\<D>) \<in> perfectly_shared_vars_rel\<close> \<open>(xs, xs') \<in>  \<langle>\<langle>Id\<rangle>list_rel\<times>\<^sub>rId\<rangle>list_rel\<close>
+  shows \<open>import_polyS \<A> xs \<le> \<Down> {((mem, xs\<^sub>0, \<A>), (mem', ys\<^sub>0, \<A>')). mem = mem' \<and> 
+    (\<A>, \<A>') \<in> perfectly_shared_vars_rel \<and>  (\<not>alloc_failed mem \<longrightarrow> (xs\<^sub>0, ys\<^sub>0) \<in> \<langle>perfectly_shared_monom \<A> \<times>\<^sub>r Id\<rangle>list_rel)}
+    (import_poly \<V>\<D> xs')\<close>
+  using assms
+  unfolding import_poly_def import_polyS_def
+  apply (refine_rcg WHILET_refine[where
+    R = \<open>{((mem, zs, xs\<^sub>0, \<A>), (mem', zs', ys\<^sub>0, \<A>')). mem = mem' \<and> 
+    (\<A>, \<A>') \<in> perfectly_shared_vars_rel \<and> (zs, zs') \<in> \<langle>\<langle>Id\<rangle>list_rel \<times>\<^sub>r Id\<rangle>list_rel
+    \<and> (\<not>alloc_failed mem \<longrightarrow> (xs\<^sub>0, ys\<^sub>0) \<in> \<langle>perfectly_shared_monom \<A> \<times>\<^sub>r Id\<rangle>list_rel)}\<close>]
+    import_monomS_import_monom)
+  subgoal by auto
+  subgoal by auto
+  subgoal by auto
+  subgoal by auto
+  subgoal by auto
+  subgoal by auto
+  subgoal by (force simp: list_rel_append1)
+  subgoal for x x' x1 x2 x1a x2a x1b x2b x1c x2c x1d x2d x1e x2e x1f x2f x1g x2g xa x'a x1h x2h x1i x2i
+    x1j x2j x1k x2k
+    using memory_allocation.exhaust_disc[of x1h \<open>x1h = Allocated\<close>]
+    by (auto intro!: list_rel_append_single intro: list_rel_mono)
+  subgoal by auto
+    done
+
+
+
+definition drop_content :: \<open>'string \<Rightarrow> ('nat, 'string) vars \<Rightarrow> ('nat, 'string) vars nres\<close>
+  where
+  \<open>drop_content = (\<lambda>v \<V>'. do {
+    ASSERT(v \<in># \<V>');
+    RETURN (remove1_mset v \<V>')
+  })\<close>
+
+
+definition drop_contentS :: \<open>'string \<Rightarrow> ('nat, 'string) shared_vars \<Rightarrow> ('nat, 'string) shared_vars nres\<close>
+  where
+  \<open>drop_contentS = (\<lambda>v (\<D>, \<V>, \<V>'). do {
+    ASSERT(v \<in># dom_m \<V>');
+    if count \<D> v = 1
+    then do {
+      let i = \<V>' \<propto> v;
+      RETURN (remove1_mset v \<D>, fmdrop i \<V>, fmdrop v \<V>')
+    }
+    else
+    RETURN (remove1_mset v \<D>, \<V>, \<V>')
+  })\<close>
+
+lemma drop_contentS_drop_content:
+  assumes \<open>(\<A>, \<V>\<D>) \<in> perfectly_shared_vars_rel\<close> \<open>(v, v') \<in> Id\<close> 
+  shows \<open>drop_contentS v \<A> \<le> \<Down>perfectly_shared_vars_rel (drop_content v' \<V>\<D>)\<close>
+proof -
+  have [simp]: \<open>count xs x = 1 \<Longrightarrow> y \<in># remove1_mset x xs \<longleftrightarrow> y \<in># xs \<and> x \<noteq>y\<close> for x xs y
+    by (auto simp add: in_diff_count)
+  have [simp]: \<open>count xs x \<noteq> 1 \<Longrightarrow> x \<in># xs \<Longrightarrow> y \<in># remove1_mset x xs \<longleftrightarrow> y \<in># xs\<close> for x xs y
+    by (metis One_nat_def add_mset_remove_trivial_eq count_add_mset count_inI in_remove1_mset_neq)
+  show ?thesis
+    using assms
+    unfolding drop_content_def drop_contentS_def
+    apply refine_vcg
+    apply (auto simp: perfectly_shared_vars_rel_def perfectly_shared_vars_def
+      distinct_mset_dom distinct_mset_remove1_All)
+    by (metis option.inject)
+qed
 end
